some progress on modexp_var_0

otbn_model/code/montmul_lemmas.dfy
@@ -10,19 +10,6 @@ module montmul_lemmas {
     import opened congruences
     import opened mont_loop_lemmas
 
-    function seq_zero(len: nat): (zs: seq<uint256>)
-        ensures |zs| == len
-    {
-        if len == 0 then []
-        else seq_zero(len - 1) + [0]
-    }
-
-    lemma seq_zero_to_nat_lemma(len: nat)
-        ensures to_nat(seq_zero(len)) == 0
-    {
-        reveal to_nat();
-    }
-
     lemma montmul_inv_lemma_0(
         a: seq<uint256>,
         x: seq<uint256>, 
