otbn_model/spec/vt_ops.dfy
@@ -15,7 +15,8 @@ module vt_ops {
 
     datatype reg32_t = GPR(index: reg_index)
 
-    type gprs_t = gprs : seq<uint32> | |gprs| == 32 witness *
+    type gprs_t = gprs : seq<uint32>
+        | |gprs| == 32 witness *
 
     datatype reg256_t =
         | WDR(index: reg_index)
@@ -28,7 +29,35 @@ module vt_ops {
         r.WDR?
     }
 
-    type wdrs_t = wdrs : seq<uint256> | |wdrs| == 32 witness *
+    type wdrs_t = wdrs : seq<uint256>
+        | |wdrs| == 32 witness *
+
+/* wdr_view definion (SHADOW) */
+
+    datatype uint512_raw = uint512_cons(
+        lh: uint256, uh: uint256, full: uint512)
+
+	type uint512_view_t = num: uint512_raw |
+		&& num.lh == uint512_lh(num.full)
+		&& num.uh == uint512_uh(num.full)
+		witness *
+
+    predicate valid_uint512_view(
+        wdrs: wdrs_t, num: uint512_view_t,
+        li: int, ui: int)
+        requires -1 <= li < BASE_5;
+        requires -1 <= ui < BASE_5;
+    {
+        && (li == NA || wdrs[li] == num.lh)
+        && (ui == NA || wdrs[ui] == num.uh)
+    }
+
+    predicate valid_wdr_view(wdrs: wdrs_t, slice: seq<uint256>, start: nat, len: nat)
+    {   
+        && |slice| == len
+        && start + len <= 32
+        && wdrs[start..start+len] == slice
+    }
 
 /* flags definions */
 
@@ -57,11 +86,59 @@ module vt_ops {
 
 /* memory definions */
 
+    type xmem_t = map<int, uint32>
+
+    predicate valid_xmem_addr(xmem: xmem_t, addr:int)
+    {
+        && addr in xmem
+    }
+
     type wmem_t = map<int, seq<uint256>>
 
-    predicate valid_xmem_addr(h: map<int, uint32>, addr:int)
+    predicate valid_wmem_base_addr(wmem: wmem_t, addr: int, size: nat)
     {
-        addr in h
+        && addr in wmem
+        && |wmem[addr]| == size != 0
+        // buff does not extend beyond mem limit
+        && addr + 32 * size <= DMEM_LIMIT
+    }
+
+/* iter_t definion (SHADOW) */
+
+    datatype iter_t = iter_cons(base_addr: int, index: nat, buff: seq<uint256>)
+
+    function bn_lid_next_iter(iter: iter_t, inc: bool): iter_t
+    {
+        iter.(index := if inc then iter.index + 1 else iter.index)
+    }
+
+    predicate iter_mapped(iter: iter_t, address: int)
+    {   
+        // we choose to ingore
+        || (address == NA)
+        // address is correct
+        || (address == iter.base_addr + 32 * iter.index)
+    }
+
+    predicate iter_inv(iter: iter_t, wmem: wmem_t, address: int)
+    {
+        var base_addr := iter.base_addr;
+        // base_addr points to a valid buffer
+        && valid_wmem_base_addr(wmem, base_addr, |iter.buff|)
+        // the view is consistent with wmem
+        && wmem[base_addr] == iter.buff
+
+        // the index is within bound (or at end)
+        && iter.index <= |iter.buff|
+        // address is correct
+        && iter_mapped(iter, address)
+    }
+
+    predicate iter_safe(iter: iter_t, wmem: wmem_t, address: int)
+    {
+        && iter_inv(iter, wmem, address)
+        // stronger constraint so we can dereference
+        && iter.index < |iter.buff|
     }
 
 /* state definions */
@@ -76,14 +153,15 @@ module vt_ops {
 
         fgroups: fgroups_t,
 
-        xmem: map<int, uint32>,
+        xmem: xmem_t,
         wmem: wmem_t,
 
         ok: bool)
     {
         function eval_reg32(r: reg32_t) : uint32
         {
-            gprs[r.index]
+            if r.index == 0 then 0
+            else gprs[r.index]
         }
 
         function eval_reg256(r: reg256_t) : uint256
@@ -328,67 +406,6 @@ module vt_ops {
             case While(cond, body) => eval_while(body, eval_cond(s, cond), s, r)
     }
 
-/* auxiliary definions */
 
-    datatype uint512_raw = uint512_cons(
-        lh: uint256, uh: uint256, full: uint512)
 
-	type uint512_view_t = num: uint512_raw |
-		&& num.lh == uint512_lh(num.full)
-		&& num.uh == uint512_uh(num.full)
-		witness *
-
-    predicate valid_uint512_view(
-        wdrs: wdrs_t, num: uint512_view_t,
-        li: int, ui: int)
-        requires -1 <= li < BASE_5;
-        requires -1 <= ui < BASE_5;
-    {
-        && (li == NA || wdrs[li] == num.lh)
-        && (ui == NA || wdrs[ui] == num.uh)
-    }
-
-    predicate valid_wdr_view(wdrs: wdrs_t, slice: seq<uint256>, start: nat, len: nat)
-    {   
-        && |slice| == len
-        && start + len <= 32
-        && wdrs[start..start+len] == slice
-    }
-
-    datatype iter_t = iter_cons(base_addr: int, index: nat, buff: seq<uint256>)
-
-    function bn_lid_next_iter(iter: iter_t, inc: bool): iter_t
-    {
-        iter.(index := if inc then iter.index + 1 else iter.index)
-    }
-
-    predicate iter_mapped(iter: iter_t, address: int)
-    {   
-        // we choose to ingore
-        || (address == NA)
-        // address is correct
-        || (address == iter.base_addr + 32 * iter.index)
-    }
-
-    predicate iter_inv(iter: iter_t, wmem: wmem_t, address: int)
-    {
-        var base_addr := iter.base_addr;
-        // base_addr points to a valid buffer
-        && base_addr in wmem
-        // the view is consistent with wmem
-        && wmem[base_addr] == iter.buff
-        // buff does not extend beyond mem limit
-        && base_addr + 32 * |iter.buff| <= DMEM_LIMIT
-        // the index is within bound (or at end)
-        && iter.index <= |iter.buff| != 0
-        // address is correct
-        && iter_mapped(iter, address)
-    }
-
-    predicate iter_safe(iter: iter_t, wmem: wmem_t, address: int)
-    {
-        && iter_inv(iter, wmem, address)
-        // stronger constraint so we can dereference
-        && iter.index < |iter.buff|
-    }
 }
